src/ByteStringHeap.v
@@ -26,6 +26,99 @@ Record PS := makePS {
   psLength : Size
 }.
 
+Definition buffer_to_list (h : Rep HeapSpec * PS) : list Word :=
+  let r   := snd h in
+  let len := psLength r in
+  let off := psBuffer r + psOffset r in
+  N.peano_rec _ []
+    (fun k ws => match M.find (off + len - N.succ k) (bytes (fst h)) with
+                 | Some w => w
+                 | None   => Zero
+                 end :: ws) len.
+
+Example buffer_to_list_ex1 :
+  buffer_to_list
+    ({| resvs := M.add 0 2 (M.empty _)
+      ; bytes := M.add 0 (Ascii.ascii_of_nat 1)
+                       (M.add 1 (Ascii.ascii_of_nat 2)
+                              (M.add 2 (Ascii.ascii_of_nat 3)
+                                     (M.empty _))) |},
+     {| psBuffer := 0
+      ; psBufLen := 3
+      ; psOffset := 0
+      ; psLength := 3 |})
+    = [ Ascii.ascii_of_nat 1
+      ; Ascii.ascii_of_nat 2
+      ; Ascii.ascii_of_nat 3 ].
+Proof.
+  unfold buffer_to_list; simpl.
+
+  rewrite F.add_eq_o; auto.
+
+  rewrite F.add_neq_o; [|nomega].
+  rewrite F.add_eq_o; auto.
+
+  rewrite F.add_neq_o; [|nomega].
+  rewrite F.add_neq_o; [|nomega].
+  rewrite F.add_eq_o; auto.
+Qed.
+
+(*
+Program Definition buffer_of_list (h : Rep HeapSpec) (xs : list Word) :
+  Comp (Rep HeapSpec * PS) :=
+  let len := N.of_nat (length xs) in
+  If 0 <? len
+  Then
+    a <- find_free_block len (resvs h);
+    ret ({| resvs := M.add a len (resvs h)
+          ; bytes :=
+              fst (fold_left (fun (z : M.t Word * Ptr Word) x =>
+                                let (h, a) := z in
+                                (M.add a x h, N.succ a))
+                             xs (bytes h, a)) |},
+         {| psBuffer := a
+          ; psBufLen := len
+          ; psOffset := 0
+          ; psLength := len |})
+  Else
+    ret (h, {| psBuffer := 0
+             ; psBufLen := 0
+             ; psOffset := 0
+             ; psLength := 0 |}).
+
+Lemma buffer_to_of_list : forall h h' xs r,
+  buffer_of_list h xs ↝ (h', r) -> buffer_to_list h' r = xs.
+Proof.
+  intros.
+  generalize dependent r.
+  induction xs;
+  unfold buffer_of_list in *;
+  simpl in *; intros;
+  destruct_computations; tsubst; simpl in *.
+    reflexivity.
+Admitted.
+*)
+
+Definition ByteString_list_AbsR
+           (or : Rep ByteStringSpec) (nr : Rep HeapSpec * PS) :=
+  or = buffer_to_list nr /\
+  IF psBufLen (snd nr) = 0
+  then psOffset (snd nr) = 0 /\ psLength (snd nr) = 0
+  else M.MapsTo (psBuffer (snd nr)) (psBufLen (snd nr)) (resvs (fst nr))
+         /\ psOffset (snd nr) + psLength (snd nr) <= psBufLen (snd nr).
+
+Ltac destruct_AbsR H :=
+  let H1 := fresh "H1" in
+  let H2 := fresh "H2" in
+  let H3 := fresh "H3" in
+  let H4 := fresh "H4" in
+  destruct H as [H1 [[H2 [H3 H4]]|[H2 [H3 H4]]]];
+  [ rewrite ?H2, ?H3, ?H4 in * | ]; subst.
+
+Ltac construct_AbsR := split; try split; simpl; try nomega.
+
+(**************************************************************************)
+
 Definition simply_widen_region (r : PS) (n : N) : PS :=
   {| psBuffer := psBuffer r
    ; psBufLen := psBufLen r
@@ -97,48 +190,7 @@ Obligation 1. nomega_. Defined.
 Obligation 2. nomega_. Defined.
 Obligation 3. nomega_. Defined.
 
-Definition buffer_uncons (h : Rep HeapSpec) (r : PS) :
-  Comp ((Rep HeapSpec * PS) * option Word) :=
-  If 0 <? psLength r
-  Then (
-    w <- peek h (psBuffer r + psOffset r);
-    ret (h, {| psBuffer := psBuffer r
-             ; psBufLen := psBufLen r
-             ; psOffset := if psLength r =? 1
-                           then 0
-                           else psOffset r + 1
-             ; psLength := psLength r - 1 |}, Some (snd w)))
-  Else ret ((h, r), None).
-
-Definition ByteString_list_AbsR
-           (or : Rep ByteStringSpec) (nr : Rep HeapSpec * PS) :=
-  let ps := snd nr in
-  length or = N.to_nat (psLength ps) /\
-  IF psBufLen ps = 0
-  then psOffset ps = 0 /\ psLength ps = 0
-  else fits (psBuffer ps) (psBufLen ps)
-            (psBuffer ps + psOffset ps) (psLength ps) /\
-       M.MapsTo (psBuffer ps) (psBufLen ps) (resvs (fst nr)) /\
-       (forall i, i < psLength ps
-          -> forall x, nth (N.to_nat i) or x = x
-          -> forall n, psBuffer ps + psOffset ps + i = n
-          -> M.MapsTo n x (bytes (fst nr))).
-
-Ltac destruct_AbsR H :=
-  let H1 := fresh "H1" in
-  let H2 := fresh "H2" in
-  destruct H as [H1 H2];
-  let H0 := fresh "H0" in
-  let H3 := fresh "H3" in
-  let H4 := fresh "H4" in
-  let H5 := fresh "H5" in
-  let data := fresh "data" in
-  destruct H2 as [[H0 [H5 H3]]|[H0 [H5 [H3 H4]]]];
-  [ rewrite ?H0, ?H5 in * |].
-
-Ltac construct_AbsR := split; try split; simpl; try nomega.
-
-Ltac if_computes_to_inv :=
+Local Ltac if_computes_to_inv :=
   match goal with
     [ H : (If ?B Then _ Else _) ↝ _ |- _ ] =>
     let Heqe := fresh "Heqe" in
@@ -147,32 +199,165 @@ Ltac if_computes_to_inv :=
     computes_to_inv
   end.
 
-Tactic Notation "by" tactic(H) :=
-  H; first [ tauto
-           | discriminate
-           | auto
-           | congruence
-           | eauto
-           | intuition
-           | firstorder ].
-
-Ltac reduce_peano i :=
-  destruct i using N.peano_ind;
-  [ left; nomega
-  | right; split; [nomega|] ];
-  try rewrite N2Nat.inj_succ in *.
-
-Ltac prepare_AbsR AbsR :=
-  destruct_computations; simpl in *;
-  destruct_AbsR AbsR; construct_AbsR;
-  right; split; [nomega|]; split; [nomega|];
-  split; trivial; intros; simplify_maps.
-
 Corollary If_Then_Else_MapsTo : forall b k k' elt (e : elt) r,
   (If b
    Then M.MapsTo k  e r
    Else M.MapsTo k' e r) = M.MapsTo (If b Then k Else k') e r.
 Proof. destruct b; trivial. Qed.
+
+Lemma Npeano_rec_eq : forall (P : N -> Set) (z : P 0) f g n,
+  (forall k x y, k < n -> x = y -> f k x = g k y)
+    -> N.peano_rec P z f n = N.peano_rec P z g n.
+Proof.
+  intros.
+  destruct n using N.peano_ind.
+    reflexivity.
+  rewrite !N.peano_rec_succ.
+  apply H.
+    nomega.
+  apply IHn.
+  intros; subst.
+  apply H.
+    nomega.
+  reflexivity.
+Qed.
+
+Lemma buffer_cons_eq_shift_1 : forall x r_n buflen,
+  0 < psOffset (snd r_n)
+    -> psBufLen (snd r_n) <= buflen
+    -> x :: buffer_to_list r_n
+         = buffer_to_list
+             ({| resvs := resvs (fst r_n)
+               ; bytes :=
+                   M.add (psBuffer (snd r_n) + (psOffset (snd r_n) - 1)) x
+                         (bytes (fst r_n)) |},
+              {| psBuffer := psBuffer (snd r_n)
+               ; psBufLen := buflen
+               ; psOffset := psOffset (snd r_n) - 1
+               ; psLength := psLength (snd r_n) + 1 |}).
+Proof.
+  intros.
+  unfold buffer_to_list; simpl.
+  destruct r_n, p; simpl in *.
+  generalize dependent buflen.
+  destruct psLength0 using N.peano_ind; simpl; intros.
+    rewrite F.add_eq_o; nomega.
+  clear IHpsLength0.
+  rewrite N.add_1_r, !N.peano_rec_succ, !N.add_sub, F.add_eq_o; trivial.
+  rewrite F.add_neq_o; [|nomega].
+  replace (psBuffer0 + (psOffset0 - 1)
+             + N.succ (N.succ psLength0) - N.succ psLength0)
+     with (psBuffer0 + psOffset0) by nomega.
+  do 2 f_equal.
+  apply Npeano_rec_eq with (P:= fun _ : N => list Word).
+  intros; subst.
+  f_equal.
+  replace (psBuffer0 + (psOffset0 - 1) + N.succ (N.succ psLength0) - N.succ k)
+     with (psBuffer0 + psOffset0 + N.succ psLength0 - N.succ k) by nomega.
+  cut (forall k, k < psLength0 ->
+          M.find (psBuffer0 + psOffset0 + N.succ psLength0 - N.succ k)
+                 (bytes r)
+            = M.find (psBuffer0 + psOffset0 + N.succ psLength0 - N.succ k)
+                     (M.add (psBuffer0 + (psOffset0 - 1)) x (bytes r))).
+    intro H3; rewrite H3; trivial.
+  intros.
+  rewrite F.add_neq_o; trivial.
+  nomega.
+Qed.
+
+Lemma buffer_cons_eq_grow_1 : forall x r_n buflen,
+  0 = psOffset (snd r_n)
+    -> psBufLen (snd r_n) <= buflen
+    -> x :: buffer_to_list r_n
+         = buffer_to_list
+             ({| resvs := resvs (fst r_n)
+               ; bytes :=
+                   M.add (psBuffer (snd r_n)) x
+                         (copy_bytes (psBuffer (snd r_n))
+                                     (psBuffer (snd r_n) + 1)
+                                     (psLength (snd r_n))
+                                     (bytes (fst r_n))
+                                     (bytes (fst r_n))) |},
+              {| psBuffer := psBuffer (snd r_n)
+               ; psBufLen := buflen
+               ; psOffset := 0
+               ; psLength := psLength (snd r_n) + 1 |}).
+Proof.
+  intros.
+  unfold buffer_to_list; simpl.
+  destruct r_n, p; simpl in *.
+  destruct psLength0 using N.peano_ind; simpl; intros.
+    rewrite F.add_eq_o; nomega.
+  subst; clear IHpsLength0.
+  rewrite N.add_1_r, !N.peano_rec_succ, !N.add_sub,
+          N.add_0_r, F.add_eq_o; [|nomega].
+  rewrite F.add_neq_o; [|nomega].
+  f_equal.
+  rewrite <- !N.add_1_r.
+  rewrite (N.add_comm (psLength0 + 1) 1).
+  rewrite N.add_assoc, N.add_assoc, N.add_sub.
+  rewrite copy_bytes_find_at; [|nomega].
+  f_equal.
+  apply Npeano_rec_eq with (P:= fun _ : N => list Word).
+  intros; subst.
+  f_equal.
+  rewrite F.add_neq_o; [|nomega].
+  rewrite copy_bytes_find.
+  destruct (within_bool (psBuffer0 + 1) (psLength0 + 1)
+                        (psBuffer0 + 1 + (psLength0 + 1) - N.succ k))
+    eqn:Heqe; simpl.
+    replace (psBuffer0 + 1 + (psLength0 + 1) - N.succ k - (psBuffer0 + 1) + psBuffer0)
+       with (psBuffer0 + psLength0 + 1 - N.succ k) by nomega.
+    reflexivity.
+  nomega.
+Qed.
+
+Lemma buffer_cons_eq_alloc_new : forall x y r_n,
+  0 = psOffset (snd r_n)
+    -> y <> psBuffer (snd r_n)
+    -> x :: buffer_to_list r_n
+         = buffer_to_list
+             ({| resvs :=
+                   M.remove (psBuffer (snd r_n))
+                            (M.add y (psLength (snd r_n) + 1)
+                                   (resvs (fst r_n)))
+               ; bytes :=
+                   M.add y x (copy_bytes (psBuffer (snd r_n)) (y + 1)
+                                         (psLength (snd r_n))
+                                         (bytes (fst r_n))
+                                         (bytes (fst r_n))) |},
+              {| psBuffer := y
+               ; psBufLen := psLength (snd r_n) + 1
+               ; psOffset := 0
+               ; psLength := psLength (snd r_n) + 1 |}).
+Proof.
+  intros.
+  unfold buffer_to_list; simpl.
+  destruct r_n, p; simpl in *.
+  destruct psLength0 using N.peano_ind; simpl; intros.
+    rewrite F.add_eq_o; nomega.
+  subst; clear IHpsLength0.
+  rewrite N.add_1_r, !N.peano_rec_succ, !N.add_sub,
+          N.add_0_r, F.add_eq_o; [|nomega].
+  rewrite F.add_neq_o; [|nomega].
+  f_equal.
+  rewrite N.add_0_r, <- !N.add_1_r.
+  rewrite (N.add_comm (psLength0 + 1) 1).
+  rewrite !N.add_assoc, <- (N.add_assoc (y + 1) psLength0 1).
+  rewrite N.add_sub, copy_bytes_find_at; [|nomega].
+  f_equal.
+  apply Npeano_rec_eq with (P:= fun _ : N => list Word).
+  intros; subst.
+  f_equal.
+  rewrite F.add_neq_o; [|nomega].
+  rewrite copy_bytes_find.
+  destruct (within_bool (y + 1) (psLength0 + 1)
+                        (y + 1 + (psLength0 + 1) - N.succ k)) eqn:Heqe; simpl.
+    replace (y + 1 + (psLength0 + 1) - N.succ k - (y + 1) + psBuffer0)
+       with (psBuffer0 + psLength0 + 1 - N.succ k) by nomega.
+    reflexivity.
+  nomega.
+Qed.
 
 Lemma buffer_cons_sound : forall r_o r_n,
   ByteString_list_AbsR r_o r_n
@@ -180,34 +365,61 @@ Lemma buffer_cons_sound : forall r_o r_n,
     -> ByteString_list_AbsR (x :: r_o) r_n'.
 Proof.
   unfold buffer_cons, Bind2; intros ? ? AbsR ???.
-  computes_to_inv.
+  destruct_computations.
+  if_computes_to_inv; subst; simpl.
+    destruct_AbsR AbsR; construct_AbsR.
+      rewrite <- buffer_cons_eq_shift_1; nomega.
+    right; intuition; nomega.
   if_computes_to_inv; subst.
-    prepare_AbsR AbsR.
-    reduce_peano i; clear IHi.
-    eapply H4; eauto; nomega.
+    destruct_computations; simpl.
+    destruct_AbsR AbsR; construct_AbsR.
+      rewrite N.add_0_r, <- buffer_cons_eq_grow_1; nomega.
+    right; intuition; nomega.
   if_computes_to_inv; subst.
-    prepare_AbsR AbsR.
-    reduce_peano i; clear IHi.
-    apply copy_bytes_mapsto.
-    destruct (within_bool _ _ n) eqn:Heqe1; simpl;
-    eapply H4; eauto; nomega.
-  if_computes_to_inv; subst.
-    prepare_AbsR AbsR.
-      split.
-        apply_for_all; nomega.
-      simplify_maps.
-    reduce_peano i; clear IHi.
-    apply copy_bytes_mapsto.
-    rewrite If_Then_Else_MapsTo.
-    apply H4 with (i:=i); try nomega.
-    assert (psOffset (snd r_n) = 0) as HA by nomega.
-    rewrite HA, !N.add_0_r in *; clear HA H6.
-    setoid_replace (n - (x1 + 1) + psBuffer (snd r_n))
-      with (psBuffer (snd r_n) + i) by nomega.
-    destruct (within_bool _ _ _) eqn:Heqe2; simpl; trivial; nomega.
-  prepare_AbsR AbsR.
-  reduce_peano i; nomega.
+    destruct_computations; simpl in *.
+    destruct_AbsR AbsR; construct_AbsR.
+      rewrite N.add_0_r, <- buffer_cons_eq_alloc_new; trivial.
+        nomega.
+      apply_for_all; nomega.
+    right.
+    split.
+      nomega.
+    split; [|nomega].
+    apply F.remove_neq_mapsto_iff; trivial.
+      apply_for_all; nomega.
+    simplify_maps.
+  destruct_computations; simpl in *.
+  destruct_AbsR AbsR; construct_AbsR.
+    unfold buffer_to_list; simpl.
+    rewrite N.add_0_r, N.add_sub, F.add_eq_o; trivial.
+    f_equal.
+    replace (psLength (snd r_n)) with 0.
+      reflexivity.
+    nomega.
+  right.
+  split.
+    nomega.
+  split.
+    simplify_maps.
+  nomega.
 Qed.
+
+(**************************************************************************)
+
+Definition buffer_uncons (h : Rep HeapSpec) (r : PS) :
+  Comp ((Rep HeapSpec * PS) * option Word) :=
+  If 0 <? psLength r
+  Then
+    `(h, w) <- peek h (psBuffer r + psOffset r);
+    ret ((h, {| psBuffer := psBuffer r
+              ; psBufLen := psBufLen r
+              ; psOffset := if psLength r =? 1
+                            then 0
+                            else psOffset r + 1
+              ; psLength := psLength r - 1 |}),
+         Some w)
+  Else
+    ret ((h, r), None).
 
 Lemma buffer_uncons_sound : forall r_o r_n a,
   ByteString_list_AbsR r_o r_n
@@ -218,35 +430,67 @@ Lemma buffer_uncons_sound : forall r_o r_n a,
                              end) (fst a).
 Proof.
   unfold buffer_uncons; intros.
-  apply refine_computes_to in H0.
-  apply refine_If_Then_Else_bool in H0.
-  destruct (0 <? psLength (snd r_n)) eqn:Heqe.
-    revert H0.
-    autorewrite with monad laws; simpl; intros.
-    apply computes_to_refine in H0.
+  if_computes_to_inv; subst; simpl.
     destruct_computations; simpl.
-    destruct_AbsR H; construct_AbsR;
-    destruct x; try destruct p; simpl in *;
-    destruct r_o; simpl in *;
-    try nomega; right;
-    split; try nomega; split;
-    destruct (psLength (snd r_n) =? 1) eqn:Heqe2;
-    try nomega;
-    try (eexists; split; [exact H4|]; nomega).
-    split; trivial; intros.
-    destruct i using N.peano_ind.
-      simpl in *.
-      rewrite N.add_0_r, N.add_assoc in H7.
-      rewrite <- H7.
-      eapply H5; eauto; nomega.
-    apply H5 with (i:=N.succ (N.succ i)); try nomega.
-    by rewrite !N2Nat.inj_succ in *.
-  apply computes_to_refine in H0.
-  destruct_computations.
-  destruct_AbsR H; construct_AbsR;
-  destruct r_o; simpl in *; auto; try nomega.
-    left; intuition.
-  right; intuition.
+    destruct_AbsR H; construct_AbsR.
+      unfold buffer_to_list.
+      destruct r_n, p; simpl.
+      destruct psLength0 using N.peano_ind; simpl; intros.
+        reflexivity.
+      rewrite !N.peano_rec_succ, <- N.pred_sub, N.pred_succ.
+      apply Npeano_rec_eq with (P:= fun _ : N => list Word).
+      intros; subst.
+      f_equal.
+      assert (N.succ psLength0 =? 1 = false) by nomega.
+      rewrite H1.
+      replace (psBuffer0 + (psOffset0 + 1) + psLength0 - N.succ k)
+         with (psBuffer0 + psOffset0 + N.succ psLength0 - N.succ k) by nomega.
+      reflexivity.
+    right; intuition;
+    destruct (psLength (@snd HeapState PS r_n) =? 1); nomega.
+  assert (psLength (@snd HeapState PS r_n) = 0) by nomega.
+  rewrite <- surjective_pairing.
+  destruct_AbsR H; construct_AbsR.
+  - unfold buffer_to_list; simpl.
+    rewrite H0; trivial.
+  - left; intuition.
+  - unfold buffer_to_list; simpl.
+    rewrite H0; trivial.
+  - right; intuition.
+Qed.
+
+Lemma buffer_to_list_cons : forall r_n,
+  0 < psLength (snd r_n) -> exists x xs, buffer_to_list r_n = x :: xs.
+Proof.
+  intros.
+  unfold buffer_to_list.
+  destruct r_n, p ; simpl in *.
+  destruct psLength0 using N.peano_ind; simpl in *; intros.
+    discriminate.
+  clear IHpsLength0.
+  rewrite N.peano_rec_succ, N.add_sub.
+  remember (N.peano_rec _ _ _ _) as xs.
+  destruct (M.find (psBuffer0 + psOffset0) (bytes r)).
+    exists w.
+    exists xs.
+    reflexivity.
+  exists Zero.
+  exists xs.
+  reflexivity.
+Qed.
+
+Lemma buffer_to_list_nil : forall r_n,
+  0 = psLength (snd r_n) -> buffer_to_list r_n = [].
+Proof.
+  intros.
+  unfold buffer_to_list.
+  destruct r_n, p ; simpl in *.
+  destruct psLength0 using N.peano_ind; simpl in *; intros.
+    reflexivity.
+  clear IHpsLength0.
+  rewrite N.peano_rec_succ, N.add_sub.
+  remember (N.peano_rec _ _ _ _) as xs.
+  destruct (M.find (psBuffer0 + psOffset0) (bytes r)); nomega.
 Qed.
 
 Lemma buffer_uncons_impl : forall r_o r_n a,
@@ -258,32 +502,43 @@ Lemma buffer_uncons_impl : forall r_o r_n a,
                end.
 Proof.
   unfold buffer_uncons; intros.
-  apply refine_computes_to in H0.
-  apply refine_If_Then_Else_bool in H0.
-  destruct (0 <? psLength (snd r_n)) eqn:Heqe.
-    revert H0.
-    autorewrite with monad laws; simpl; intros.
-    apply computes_to_refine in H0.
-    destruct_computations.
-    destruct_AbsR H; simpl;
-    destruct r_o; simpl in *; try nomega.
-    f_equal; tsubst.
-    apply H0.
-    replace (psBuffer (snd r_n) + psOffset (snd r_n))
-       with (psBuffer (snd r_n) + psOffset (snd r_n) + 0) by nomega.
-    eapply H5; eauto; nomega.
-  apply computes_to_refine in H0.
-  apply Return_inv in H0.
-  destruct a; tsubst; simpl in *.
-  destruct r_o; simpl in *;
-  destruct H, H0; auto.
-    destruct H0, H1.
-    rewrite H2 in H; simpl in H.
-    discriminate.
+  destruct H; subst.
+  clear H1.
+  if_computes_to_inv; subst; simpl.
+    destruct_computations; simpl.
+    assert (0 < psLength (snd r_n)) by nomega.
+    apply buffer_to_list_cons in H0.
+    destruct H0, H0.
+    rewrite H0.
+    f_equal.
+    unfold buffer_to_list in H0.
+    destruct r_n, p; simpl in *.
+    destruct psLength0 using N.peano_ind; simpl in *; intros.
+      discriminate.
+    clear IHpsLength0.
+    rewrite N.peano_rec_succ, N.add_sub in H0.
+    inv H0.
+    destruct H.
+      apply F.find_mapsto_iff in H.
+      rewrite H.
+      reflexivity.
+    destruct H; subst.
+    assert (M.find (psBuffer0 + psOffset0) (bytes r) = None).
+      apply F.not_find_in_iff.
+      assumption.
+    rewrite H0.
+    reflexivity.
+  unfold buffer_to_list; simpl.
+  destruct r_n, p; simpl.
+  destruct psLength0 using N.peano_ind; simpl in *; intros; trivial.
+  rewrite N.peano_rec_succ, N.add_sub.
   nomega.
 Qed.
 
+(**************************************************************************)
+
 (* jww (2016-12-21): For now, just allocate and copy from both. *)
+
 Program Definition buffer_append
         (h1 : Rep HeapSpec) (r1 : PS)
         (h2 : Rep HeapSpec) (r2 : PS) :
@@ -295,9 +550,10 @@ Program Definition buffer_append
       `(h1, a) <- alloc h1 (psLength r1 + psLength r2);
       h1 <- memcpy h1 (psBuffer r1 + psOffset r1) a (psLength r1);
       let h1 := {| resvs := resvs h1
-                 ; bytes := copy_bytes_between_heaps
-                              (psBuffer r2 + psOffset r2) a (psLength r2)
-                              (bytes h2) (bytes h1) |} in
+                 ; bytes :=
+                     copy_bytes (psBuffer r2 + psOffset r2)
+                                (a + psLength r1) (psLength r2)
+                                (bytes h2) (bytes h1) |} in
       ret (h1, {| psBuffer := a
                 ; psBufLen := psLength r1 + psLength r2
                 ; psOffset := 0
@@ -305,13 +561,6 @@ Program Definition buffer_append
     Else fun _ => ret (h1, r1)
   Else fun _ => ret (h2, r2).
 Obligation 1. nomega. Defined.
-
-Lemma refineEquiv_If_Then_Else :
-  forall (A : Type) (c : bool) (x y : Comp A),
-    refineEquiv x y ->
-    forall x0 y0 : Comp A, refineEquiv x0 y0 ->
-    refineEquiv (If c Then x Else x0) (If c Then y Else y0).
-Proof. intros; destruct c; auto. Qed.
 
 Lemma refineEquiv_buffer_append
       (h1 : Rep HeapSpec) (r1 : PS)
@@ -326,9 +575,10 @@ Lemma refineEquiv_buffer_append
                        ; bytes := bytes h1 |}
                       (psBuffer r1 + psOffset r1) x0 (psLength r1);
          ret ({| resvs := resvs h0
-               ; bytes := copy_bytes_between_heaps
-                            (psBuffer r2 + psOffset r2) x0 (psLength r2)
-                            (bytes h2) (bytes h0) |},
+               ; bytes :=
+                   copy_bytes (psBuffer r2 + psOffset r2)
+                              (x0 + psLength r1) (psLength r2)
+                              (bytes h2) (bytes h0) |},
               {| psBuffer := x0
                ; psBufLen := psLength r1 + psLength r2
                ; psOffset := 0
@@ -366,6 +616,134 @@ Proof.
   reflexivity.
 Qed.
 
+Lemma buffer_to_list_app : forall r_n1 r_n2 v,
+  buffer_to_list r_n1 ++ buffer_to_list r_n2 =
+  buffer_to_list
+    ({|
+     resvs := M.add v (psLength (snd r_n1) + psLength (snd r_n2))
+                    (resvs (fst r_n1));
+     bytes :=
+       copy_bytes (psBuffer (snd r_n2) + psOffset (snd r_n2))
+                  (v + psLength (snd r_n1))
+                  (psLength (snd r_n2))
+                  (bytes (fst r_n2))
+                  (copy_bytes (psBuffer (snd r_n1) + psOffset (snd r_n1)) v
+                              (psLength (snd r_n1))
+                              (bytes (fst r_n1)) (bytes (fst r_n1))) |},
+    {|
+    psBuffer := v;
+    psBufLen := psLength (snd r_n1) + psLength (snd r_n2);
+    psOffset := 0;
+    psLength := psLength (snd r_n1) + psLength (snd r_n2) |}).
+Proof.
+  intros.
+  destruct r_n1, p; simpl.
+  destruct r_n2, p; simpl.
+  destruct psLength0 using N.peano_ind; simpl in *; intros; trivial;
+  try clear IHpsLength0;
+  destruct psLength1 using N.peano_ind; simpl in *; intros; trivial;
+  try clear IHpsLength1.
+  - rewrite N.add_0_r.
+    unfold buffer_to_list; simpl.
+    apply Npeano_rec_eq with (P:= fun _ : N => list Word).
+    intros; subst; f_equal.
+    rewrite N.add_0_r, !copy_bytes_find.
+    assert (within_bool v 0 (v + N.succ psLength1 - N.succ k) = false)
+      by nomega.
+    rewrite H0; clear H0; simpl.
+    assert (within_bool v (N.succ psLength1)
+                        (v + N.succ psLength1 - N.succ k) = true)
+      by nomega.
+    rewrite H0; clear H0; simpl.
+    replace (v + N.succ psLength1 - N.succ k - v + (psBuffer1 + psOffset1))
+       with (psBuffer1 + psOffset1 + N.succ psLength1 - N.succ k)
+         by nomega.
+    reflexivity.
+  - remember (r0, _) as b.
+    rewrite (buffer_to_list_nil b), app_nil_r, !N.add_0_r; [|nomega].
+    clear Heqb b.
+    unfold buffer_to_list; simpl.
+    destruct psLength0 using N.peano_ind; simpl; intros.
+      rewrite !N.add_sub, N.add_0_r, !copy_bytes_find.
+      assert (within_bool (v + 1) 0 v = false) by nomega.
+      rewrite H; clear H; simpl.
+      assert (within_bool v 1 v = true) by nomega.
+      rewrite H; clear H; simpl.
+      replace (v - v + (psBuffer0 + psOffset0))
+         with (psBuffer0 + psOffset0) by nomega.
+      reflexivity.
+    subst; clear IHpsLength0.
+    apply Npeano_rec_eq with (P:= fun _ : N => list Word).
+    intros; subst; f_equal.
+    rewrite N.add_0_r, !copy_bytes_find.
+    assert (within_bool (v + N.succ (N.succ psLength0)) 0
+                        (v + N.succ (N.succ psLength0) - N.succ k) = false)
+      by nomega.
+    rewrite H0; clear H0; simpl.
+    assert (within_bool v (N.succ (N.succ psLength0))
+                        (v + N.succ (N.succ psLength0) - N.succ k) = true)
+      by nomega.
+    rewrite H0; clear H0; simpl.
+    replace (v + N.succ (N.succ psLength0) - N.succ k - v + (psBuffer0 + psOffset0))
+       with (psBuffer0 + psOffset0 + N.succ (N.succ psLength0) - N.succ k)
+         by nomega.
+    reflexivity.
+  - unfold buffer_to_list; simpl.
+    rewrite !N.peano_rec_succ, N.add_sub.
+    rewrite N.add_succ_l.
+    rewrite <- (N.add_succ_comm psLength0 psLength1).
+    rewrite !N.peano_rec_succ, N.add_sub.
+    rewrite N.add_succ_l.
+    rewrite N.peano_rec_succ, N.add_sub.
+    rewrite !N.add_0_r, !copy_bytes_find.
+    assert (within_bool (v + N.succ psLength0) (N.succ psLength1) v = false)
+      by nomega.
+    rewrite H; clear H; simpl.
+    assert (within_bool v (N.succ psLength0) v = true) by nomega.
+    rewrite H; clear H; simpl.
+    replace (v - v + (psBuffer0 + psOffset0)) with (psBuffer0 + psOffset0)
+      by nomega.
+    f_equal.
+    replace (v + N.succ (N.succ (psLength0 + psLength1))
+               - N.succ (psLength0 + psLength1))
+       with (v + 1 + N.succ (psLength0 + psLength1)
+                   - N.succ (psLength0 + psLength1))
+         by nomega.
+    rewrite !N.add_sub.
+    destruct (within_bool (v + N.succ psLength0)
+                          (N.succ psLength1) (v + 1)) eqn:Heqe; simpl.
+      assert (0 = psLength0) by nomega.
+      subst; simpl.
+      replace (v + 1 - (v + 1) + (psBuffer1 + psOffset1))
+         with (psBuffer1 + psOffset1) by nomega.
+      f_equal.
+      apply Npeano_rec_eq with (P:= fun _ : N => list Word).
+      intros; subst; f_equal.
+      rewrite !copy_bytes_find.
+      assert (within_bool (v + 1) (N.succ psLength1)
+                          (v + N.succ (N.succ psLength1) - N.succ k) = true)
+        by nomega.
+      rewrite H0; clear H0; simpl.
+      replace (v + N.succ (N.succ psLength1) - N.succ k
+                 - (v + 1) + (psBuffer1 + psOffset1))
+         with (psBuffer1 + psOffset1 + N.succ psLength1 - N.succ k)
+           by nomega.
+      reflexivity.
+    assert (within_bool v (N.succ psLength0) (v + 1) = true) by nomega.
+    rewrite H; clear H; simpl.
+    replace (v + 1 - v + (psBuffer0 + psOffset0))
+       with (N.succ (psBuffer0 + psOffset0)) by nomega.
+    assert (psLength0 <> 0) by nomega.
+    apply N.neq_0_r in H.
+    destruct H; subst.
+    rewrite N.peano_rec_succ.
+    replace (psBuffer0 + psOffset0 + N.succ (N.succ x) - N.succ x)
+       with (N.succ (psBuffer0 + psOffset0)) by nomega.
+    rewrite <- app_comm_cons.
+    f_equal.
+    rewrite N.add_succ_l, N.peano_rec_succ, !copy_bytes_find.
+Admitted.
+
 Lemma buffer_append_sound : forall r_o1 r_o2 r_n1 r_n2,
   ByteString_list_AbsR r_o1 r_n1
     -> ByteString_list_AbsR r_o2 r_n2
@@ -376,72 +754,46 @@ Proof.
   intros.
   apply refine_computes_to in H1.
   rewrite refineEquiv_buffer_append in H1.
-  apply refine_If_Then_Else_bool in H1.
-  destruct r_n1, p; simpl in H1.
-  revert H1.
-  destruct psLength0 eqn:Heqe1; simpl; intros.
-    apply computes_to_refine in H1.
-    destruct_computations.
-    destruct_AbsR H; simpl;
-    destruct r_o1; simpl in *; try nomega.
-  destruct r_n2, p0; simpl in H1.
-  revert H1.
-  destruct psLength1 eqn:Heqe2; simpl; intros.
-    apply computes_to_refine in H1.
-    destruct_computations.
-    destruct_AbsR H0; simpl;
-    destruct r_o2; simpl in *; try nomega;
-    rewrite app_nil_r; trivial.
-  revert H1.
-  unfold find_free_block, memcpy.
-  autorewrite with monad laws; simpl.
-  intro H1.
   apply computes_to_refine in H1.
-  destruct_computations.
-  destruct_AbsR H; destruct_AbsR H0; construct_AbsR;
-  destruct r_o1, r_o2; simpl in *;
-  rewrite ?Pos2Nat.inj_add, <- ?H2, <- ?H3, ?app_length;
-  try nomega;
-  [ left; intuition;
-    rewrite <- positive_nat_N, Pos2Nat.inj_add; nomega
-  | right; intuition;
-    [ nomega
-    | rewrite <- positive_nat_N, Pos2Nat.inj_add; nomega
-    | rewrite <- !positive_nat_N, <- ?H2, <- ?H3 ] .. ].
-  - admit.
-  - admit.
-  - admit.
-Admitted.
-
-Lemma refine_skip2 {B} (dummy : Comp B) {A} (a : Comp A) :
-  refine a (dummy >> a).
-Proof.
-  repeat first [ intro
-               | computes_to_inv
-               | assumption
-                 | econstructor; eassumption
-                 | econstructor; try eassumption; [] ].
-  eauto.
+  if_computes_to_inv.
+    if_computes_to_inv.
+      subst.
+      destruct_computations; simpl in *.
+      destruct_AbsR H.
+        destruct_AbsR H0; construct_AbsR.
+      construct_AbsR.
+        destruct_AbsR H0;
+        apply buffer_to_list_app.
+      right.
+      split.
+        nomega.
+      split.
+        simplify_maps.
+      nomega.
+    rewrite <- surjective_pairing in H1.
+    subst.
+    assert (r_o2 = []).
+      destruct H0; subst.
+      destruct r_n2, p; simpl in *.
+      unfold buffer_to_list; simpl.
+      assert (psLength0 = 0) by nomega.
+      rewrite H0; simpl.
+      reflexivity.
+    rewrite H1, app_nil_r.
+    assumption.
+  assert (r_o1 = []).
+    destruct H; subst.
+    destruct r_n1, p; simpl in *.
+    unfold buffer_to_list; simpl.
+    assert (psLength0 = 0) by nomega.
+    rewrite H; simpl.
+    reflexivity.
+  rewrite <- surjective_pairing in H1.
+  rewrite H2, app_nil_l, <- H1.
+  assumption.
 Qed.
 
-Class RefineUnder {A : Type} (a a' : Comp A) := {
-  rewrite_under : refine a a'
-}.
-
-Instance RefineUnder_Bind {A B : Type}
-         (ca ca' : Comp A)
-         (b b' : A -> Comp A)
-         (refine_a : refine ca ca')
-         (refine_b : forall a, ca ↝ a -> refine (b a) (b' a)) :
-  RefineUnder (a <- ca; b a) (a' <- ca'; b' a') :=
-  {| rewrite_under := refine_under_bind_both b b' refine_a refine_b |}.
-
-Definition refine_skip2_pick {B} (dummy : Comp B) {A} (P : A -> Prop) :
-  refine {a | P a} (dummy >> {a | P a}) := @refine_skip2 _ _ _ _.
-
-Definition refine_skip2_bind {B} (dummy : Comp B)
-           {A C} (ca : Comp A) (k : A -> Comp C) :
-  refine (ca >>= k) (dummy >> (ca >>= k)) := @refine_skip2 _ _ _ _.
+(**************************************************************************)
 
 Theorem ByteStringHeap (heap : Rep HeapSpec) :
   { adt : _ & refineADT ByteStringSpec adt }.
@@ -458,6 +810,7 @@ Proof.
                       ; psOffset := 0
                       ; psLength := 0 |}).
       finish honing.
+    simpl.
     firstorder.
   }
 
