src/HeapState.v
@@ -89,24 +89,25 @@ Definition keep_range {elt} (addr : M.key) (len : N) : M.t elt -> M.t elt :=
 Definition drop_range {elt} (addr : M.key) (len : N) : M.t elt -> M.t elt :=
   keep_keys (fun p => negb (within_bool addr len p)).
 
-Definition copy_bytes {elt} (from to : M.key) (len : N) (m : M.t elt) :
-  M.t elt :=
-  P.update (drop_range to len m)
+Definition copy_bytes {elt} (from to : M.key) (len : N)
+           (mfrom mto : M.t elt) : M.t elt :=
+  P.update (drop_range to len mto)
            (M.fold (fun k e rest =>
                       If within_bool from len k
                       Then M.add (k - from + to) e rest
                       Else rest)
-                   m (M.empty _)).
+                   mfrom (M.empty _)).
 
 Program Instance copy_bytes_Proper :
-  Proper (eq ==> eq ==> eq ==> M.Equal ==> @M.Equal elt) copy_bytes.
+  Proper (eq ==> eq ==> eq ==> M.Equal ==> M.Equal ==> @M.Equal elt)
+         copy_bytes.
 Obligation 1.
   relational.
   unfold copy_bytes, drop_range, keep_range, keep_keys.
   apply P.update_m; trivial.
-    rewrite H2; reflexivity.
+    rewrite H3; reflexivity.
   apply P.fold_Equal; eauto; relational.
-  - destruct (within_bool y y1 y3); simpl;
+  - destruct (within_bool y y1 y4); simpl;
     rewrite H1; reflexivity.
   - intros ??????.
     destruct (within_bool y y1 k) eqn:Heqe; simpl;
@@ -119,11 +120,11 @@ Obligation 1.
     nomega.
 Qed.
 
-Lemma copy_bytes_mapsto : forall elt k (e : elt) addr1 addr2 len m,
-  M.MapsTo k e (copy_bytes addr1 addr2 len m)
+Lemma copy_bytes_mapsto : forall elt k (e : elt) addr1 addr2 len m1 m2,
+  M.MapsTo k e (copy_bytes addr1 addr2 len m1 m2)
     <-> (If within_bool addr2 len k
-         Then M.MapsTo ((k - addr2) + addr1) e m
-         Else M.MapsTo (elt:=elt) k e m).
+         Then M.MapsTo (k - addr2 + addr1) e m1
+         Else M.MapsTo (elt:=elt) k e m2).
 Proof.
   unfold copy_bytes, drop_range, keep_range, keep_keys,
          const, not, compose.
@@ -132,7 +133,7 @@ Proof.
     destruct H.
       revert H.
       apply P.fold_rec_bis; simpl; intros; intuition.
-        destruct (within_bool addr2 len k) eqn:Heqe; simpl in *;
+        destruct (within_bool addr2 len k) eqn:Heqe; simpl in *; trivial.
         rewrite <- H; assumption.
       destruct (within_bool addr2 len k) eqn:Heqe; simpl in *.
         destruct (within_bool addr1 len k0) eqn:Heqe1; simpl in *.
@@ -143,27 +144,7 @@ Proof.
         simplify_maps; right; split; [nomega|intuition].
       destruct (within_bool addr1 len k0) eqn:Heqe1; simpl in *.
         simplify_maps.
-          simplify_maps.
-          nomega.
-        simplify_maps.
-        right.
-        split.
-          specialize (H1 H6).
-          unfold not; intros; subst.
-          contradiction H0.
-          apply in_mapsto_iff.
-          exists e.
-          assumption.
-        intuition.
-      simplify_maps.
-      right.
-      split.
-        specialize (H1 H2).
-        unfold not; intros; subst.
-        contradiction H0.
-        apply in_mapsto_iff.
-        exists e.
-        assumption.
+        nomega.
       intuition.
     destruct H.
     destruct (within_bool addr2 len k) eqn:Heqe; simpl in *.
@@ -208,14 +189,86 @@ Proof.
   contradiction.
 Qed.
 
+Lemma copy_bytes_find : forall a1 a2 k l elt (m1 m2 : M.t elt),
+  M.find k (copy_bytes a1 a2 l m1 m2)
+    = If within_bool a2 l k
+      Then M.find (k - a2 + a1) m1
+      Else M.find k m2.
+Proof.
+  intros.
+  unfold copy_bytes, drop_range, keep_keys.
+  destruct (within_bool a2 l k) eqn:Heqe; simpl.
+  {
+    rewrite update_find_r.
+    apply P.fold_rec_weak; intros.
+    - rewrite <- H; assumption.
+    - rewrite !F.empty_o; trivial.
+    - destruct (within_bool a1 l k0) eqn:Heqe2; simpl.
+        destruct (N.eq_dec (k0 - a1 + a2) k); subst.
+          replace (k0 - a1 + a2 - a2 + a1) with k0 by nomega.
+          rewrite !F.add_eq_o; trivial.
+        assert (k0 <> k - a2 + a1) by nomega.
+        rewrite !F.add_neq_o; trivial.
+      assert (k0 <> k - a2 + a1) by nomega.
+      rewrite F.add_neq_o; trivial.
+    - unfold not; intros.
+      destruct (proj1 (in_mapsto_iff _ _ _) H); clear H.
+      simplify_maps; relational.
+      nomega.
+  }
+  {
+    rewrite update_find_l.
+      unfold P.filter.
+      apply P.fold_rec_weak; intros; trivial.
+        rewrite <- H; assumption.
+      destruct (N.eq_dec k0 k); subst.
+        rewrite Heqe; simpl.
+        rewrite !F.add_eq_o; trivial.
+      destruct (negb (within_bool a2 l k0));
+      rewrite !F.add_neq_o; trivial.
+    apply P.fold_rec_weak; intros; trivial;
+    unfold not; intros.
+      apply F.empty_in_iff in H; trivial.
+    destruct (within_bool a1 l k0) eqn:Heqe1; simpl in H1.
+      destruct H1.
+      simplify_maps.
+        nomega.
+      contradiction H0.
+      exists x.
+      assumption.
+    nomega.
+  }
+Qed.
+
+Lemma copy_bytes_zero {elt} addr1 addr2 (m1 m2 : M.t elt) :
+  M.Equal (elt:=elt) (copy_bytes addr1 addr2 0 m1 m2) m2.
+Proof.
+  apply F.Equal_mapsto_iff; split; intros;
+  [ apply copy_bytes_mapsto in H
+  | apply copy_bytes_mapsto ];
+  destruct (within_bool addr2 0 k) eqn:Heqe; simpl in *; trivial;
+  nomega.
+Qed.
+
 Lemma copy_bytes_idem d len elt (m : M.t elt) :
-  M.Equal (copy_bytes d d len m) m.
+  M.Equal (copy_bytes d d len m m) m.
 Proof.
   apply F.Equal_mapsto_iff; split; intros;
   [ apply copy_bytes_mapsto in H
   | apply copy_bytes_mapsto ];
   destruct (within_bool d len k) eqn:Heqe; simpl in *; trivial;
   revert H; replace (k - d + d) with k by nomega; trivial.
+Qed.
+
+Lemma copy_bytes_find_at : forall b k l elt (m1 m2 : M.t elt),
+  0 < l -> M.find k (copy_bytes b k l m1 m2) = M.find b m1.
+Proof.
+  intros.
+  rewrite copy_bytes_find.
+  assert (within_bool k l k = true) by nomega.
+  rewrite H0; simpl.
+  replace (k - k + b) with b by nomega.
+  reflexivity.
 Qed.
 
 Lemma increase_heap_ceiling : forall n m r,
@@ -235,85 +288,6 @@ Proof.
   intros.
   relational.
   destruct c; eauto.
-Qed.
-
-Definition copy_bytes_between_heaps {elt} (from to : M.key) (len : N)
-           (mfrom mto : M.t elt) : M.t elt :=
-  P.update (drop_range to len mto)
-           (M.fold (fun k e rest =>
-                      If within_bool from len k
-                      Then M.add (k - from + to) e rest
-                      Else rest)
-                   mfrom (M.empty _)).
-
-Lemma copy_bytes_between_heaps_mapsto :
-  forall elt k (e : elt) addr1 addr2 len m1 m2,
-    M.MapsTo k e (copy_bytes_between_heaps addr1 addr2 len m1 m2)
-      <-> (If within_bool addr2 len k
-           Then M.MapsTo ((k - addr2) + addr1) e m1
-           Else M.MapsTo (elt:=elt) k e m2).
-Proof.
-  unfold copy_bytes_between_heaps, drop_range, keep_range, keep_keys,
-         const, not, compose.
-  split; intros.
-    apply P.update_mapsto_iff in H.
-    destruct H.
-      revert H.
-      apply P.fold_rec_bis; simpl; intros; intuition.
-        destruct (within_bool addr2 len k) eqn:Heqe; simpl in *; trivial;
-        rewrite <- H; assumption.
-      destruct (within_bool addr2 len k) eqn:Heqe; simpl in *.
-        destruct (within_bool addr1 len k0) eqn:Heqe1; simpl in *.
-          simplify_maps.
-            simplify_maps.
-            nomega.
-          simplify_maps; right; split; [nomega|intuition].
-        simplify_maps; right; split; [nomega|intuition].
-      destruct (within_bool addr1 len k0) eqn:Heqe1; simpl in *.
-        simplify_maps.
-        nomega.
-      intuition.
-    destruct H.
-    destruct (within_bool addr2 len k) eqn:Heqe; simpl in *.
-      simplify_maps; relational.
-      nomega.
-    simplify_maps; relational.
-  apply P.update_mapsto_iff.
-  destruct (within_bool addr2 len k) eqn:Heqe; simpl in *.
-    left.
-    revert H.
-    apply P.fold_rec_bis; simpl; intros; intuition.
-      rewrite <- H in H1.
-      intuition.
-    destruct (within_bool addr1 len k0) eqn:Heqel; simpl.
-      simplify_maps.
-        simplify_maps.
-        nomega.
-      simplify_maps.
-      right.
-      split.
-        nomega.
-      intuition.
-    simplify_maps.
-    nomega.
-  right.
-  split.
-    simplify_maps; relational.
-    split; trivial.
-    nomega.
-  apply P.fold_rec_bis; simpl; intros; intuition.
-    inversion H0.
-    simplify_maps.
-  destruct (within_bool addr1 len k0) eqn:Heqel; simpl in *.
-    apply (proj1 (in_mapsto_iff _ _ _)) in H3.
-    destruct H3.
-    simplify_maps.
-      nomega.
-    contradiction H2.
-    apply in_mapsto_iff.
-    exists x.
-    assumption.
-  contradiction.
 Qed.
 
 End HeapState.
